Proofs for C06: Inductive Structures

MIL/C06_Discrete_Mathematics/S03_Inductive_Structures.lean
@@ -61,12 +61,28 @@ theorem map_map' (f : α → β) (g : β → γ) (as : List α) :
   . rfl
   . simp [map, ih]
 
-def reverse : List α → List α := sorry
+def reverse : List α → List α
+  | [] => []
+  | a :: as => reverse as ++ [a]
+
+#eval reverse [1, 2, 3, 4 , 5]
+
 
 theorem reverse_append (as bs : List α) : reverse (as ++ bs) = reverse bs ++ reverse as := by
-  sorry
+  induction' as with a as ih
 
-theorem reverse_reverse (as : List α) : reverse (reverse as) = as := by sorry
+  simp; rw [reverse]
+
+  rw [reverse]
+  rw [← append_assoc, ← ih, cons_append, reverse]
+
+
+theorem reverse_reverse (as : List α) : reverse (reverse as) = as := by
+  induction' as with a as ih
+
+  rw [reverse, reverse]
+
+  rw [reverse, reverse_append, ih, reverse, reverse, nil_append, cons_append, nil_append]
 
 end MyListSpace3
 
@@ -97,14 +113,33 @@ theorem size_le : ∀ t : BinTree, size t ≤ 2^depth t - 1
           have : 0 < 2 ^ max l.depth r.depth := by simp
           omega
 
-theorem depth_le_size : ∀ t : BinTree, depth t ≤ size t := by sorry
+theorem depth_le_size : ∀ t : BinTree, depth t ≤ size t
+  | empty     => Nat.zero_le 0
+  | node l r => by
+    simp only [depth, size]
+    calc max l.depth r.depth + 1
+      ≤ max l.size r.size + 1 := by
+          gcongr <;> apply depth_le_size
+    _ ≤ l.size + r.size + 1 := by
+          omega
 
-def flip : BinTree → BinTree := sorry
+
+def flip : BinTree → BinTree
+  | empty => empty
+  | node l r => node (flip r) (flip l)
 
 example: flip  (node (node empty (node empty empty)) (node empty empty)) =
-    node (node empty empty) (node (node empty empty) empty) := sorry
+    node (node empty empty) (node (node empty empty) empty) := rfl
 
-theorem size_flip : ∀ t, size (flip t) = size t := by sorry
+theorem size_flip : ∀ t, size (flip t) = size t
+  | empty     => rfl
+  | node l r  => by
+    simp [size, flip]
+    calc r.flip.size + l.flip.size
+      = l.size + r.size := by
+          rw [size_flip r, size_flip, add_comm]
+
+
 end BinTree
 
 inductive PropForm : Type where
@@ -152,9 +187,47 @@ def subst : PropForm → ℕ → PropForm → PropForm
   | impl A B, m, C => impl (A.subst m C) (B.subst m C)
 
 theorem subst_eq_of_not_mem_vars :
-    ∀ (A : PropForm) (n : ℕ) (C : PropForm), n ∉ A.vars → A.subst n C = A := sorry
+    ∀ (A : PropForm) (n : ℕ) (C : PropForm), n ∉ A.vars → A.subst n C = A := by
+  intro A n C nAvars
+  induction' A with n D E nD nE D E nD nE D E nD nE
+
+  simp [subst]; intro contra
+  rw [contra, vars] at nAvars
+  tauto
+
+  simp [subst]
+
+  simp [vars] at nAvars
+  rcases nAvars with ⟨n1, n2⟩
+  apply nD at n1
+  apply nE at n2
+  simp [subst]
+  exact ⟨n1, n2⟩
+
+  simp [vars] at nAvars
+  rcases nAvars with ⟨n1, n2⟩
+  apply nD at n1
+  apply nE at n2
+  simp [subst]
+  exact ⟨n1, n2⟩
+
+  simp [vars] at nAvars
+  rcases nAvars with ⟨n1, n2⟩
+  apply nD at n1
+  apply nE at n2
+  simp [subst]
+  exact ⟨n1, n2⟩
+
 
 theorem subst_eval_eq : ∀ (A : PropForm) (n : ℕ) (C : PropForm) (v : ℕ → Bool),
-  (A.subst n C).eval v = A.eval (fun m => if m = n then C.eval v else v m) := sorry
+  (A.subst n C).eval v = A.eval (fun m => if m = n then C.eval v else v m)
+  | var m, n, C, v => by
+    simp_all [subst, eval, conj, subst_eval_eq]
+    split <;> rfl
+  | fls, n, C, v => by simp_all [subst, eval, conj, subst_eval_eq]
+  | conj A B, n, C, v => by simp_all [subst, eval, conj, subst_eval_eq]
+  | disj A B, n, C, v => by simp_all [subst, eval, conj, subst_eval_eq]
+
+  | impl A B, n, C, v => by simp_all [subst, eval, conj, subst_eval_eq]
 
 end PropForm
